Prove word syn props via new not_created constant
Now update the various proofs of the word-lang syntax restrictions (proofs of
no_alloc, no_mt, no_share_inst etc) using the one pass.

compiler/backend/semantics/wordPropsScript.sml
@@ -3543,7 +3543,7 @@ Proof
   >> (unabbrev_all_tac>>EVERY_CASE_TAC>>fs[every_var_imm_def])
 QED
 
-val get_code_labels_def = Define`
+Definition get_code_labels_def[simp]:
   (get_code_labels (Call r d a h) =
     (case d of SOME x => {x} | _ => {}) ∪
     (case r of SOME (_,_,x,_,_) => get_code_labels x | _ => {}) ∪
@@ -3552,8 +3552,8 @@ val get_code_labels_def = Define`
   (get_code_labels (If _ _ _ p1 p2) = get_code_labels p1 ∪ get_code_labels p2) ∧
   (get_code_labels (MustTerminate p) = get_code_labels p) ∧
   (get_code_labels (LocValue _ l1) = {l1}) ∧
-  (get_code_labels _ = {})`;
-val _ = export_rewrites["get_code_labels_def"];
+  (get_code_labels _ = {})
+End
 
 (* TODO: This seems like it must have been established before
   handler labels point only within the current table entry
@@ -4507,18 +4507,23 @@ Definition not_created_subprogs_def:
   not_created_subprogs _ _ = T
 End
 
-Definition no_alloc_def:
-  no_alloc p = not_created_subprogs ((<>) (Alloc 0 LN)) p
+Theorem not_created_subprogs_P_def = not_created_subprogs_def
+  |> BODY_CONJUNCTS
+  |> map (fn t => GEN (hd (snd (strip_comb (lhs (concl t))))) t)
+  |> map (Q.SPEC `P`) |> LIST_CONJ
+  |> Q.GEN `P`
+
+(* no_alloc specialisation *)
+
+val no_alloc_P = ``((<>) (Alloc 0 LN))``
+
+Definition no_alloc_subprogs_def:
+  no_alloc p = not_created_subprogs ^no_alloc_P p
 End
 
-(* Sigh ... *)
-val not_created_lhs_pats = not_created_subprogs_def |> BODY_CONJUNCTS
-    |> map (snd o dest_comb o lhs o concl o SPEC_ALL)
-
-Theorem no_alloc_def2 =
-  map (fn t => REWRITE_CONV [no_alloc_def, not_created_subprogs_def] ``no_alloc ^t``)
-        not_created_lhs_pats
-    |> map (REWRITE_RULE [GSYM no_alloc_def]) |> LIST_CONJ
+Theorem no_alloc_def = not_created_subprogs_P_def
+  |> ISPEC no_alloc_P
+  |> REWRITE_RULE [GSYM no_alloc_subprogs_def]
 
 val no_alloc_code_def = Define `
   no_alloc_code (code : (num # ('a wordLang$prog)) num_map) ⇔
@@ -4536,14 +4541,15 @@ Proof
   metis_tac[]
 QED
 
-Definition no_install_def:
-  no_install p = not_created_subprogs ((<>) (Install 0 0 0 0 LN)) p
+val no_install_P = ``((<>) (Install 0 0 0 0 LN))``
+
+Definition no_install_subprogs_def:
+  no_install p = not_created_subprogs ^no_install_P p
 End
 
-Theorem no_install_def2 =
-  map (fn t => REWRITE_CONV [no_install_def, not_created_subprogs_def] ``no_install ^t``)
-        not_created_lhs_pats
-    |> map (REWRITE_RULE [GSYM no_install_def]) |> LIST_CONJ
+Theorem no_install_def = not_created_subprogs_P_def
+  |> ISPEC no_install_P
+  |> REWRITE_RULE [GSYM no_install_subprogs_def]
 
 val no_install_code_def = Define `
     no_install_code (code : (num # ('a wordLang$prog)) num_map) ⇔
@@ -4582,13 +4588,13 @@ Proof
     >- (EVERY_CASE_TAC >> fs[call_env_def, flush_state_def, dec_clock_def] >> rw[] >> fs[])
     >- (EVERY_CASE_TAC >> fs[] >> rename1 `evaluate (p, st)` >>
         Cases_on `evaluate (p, st)` >>
-        fs[no_install_def2] >> EVERY_CASE_TAC >> fs[] >> rw[] >> fs[])
-    >- (Cases_on `evaluate (c1,s)` >> fs[no_install_def2] >> CASE_TAC >> rfs[])
+        fs[no_install_def] >> EVERY_CASE_TAC >> fs[] >> rw[] >> fs[])
+    >- (Cases_on `evaluate (c1,s)` >> fs[no_install_def] >> CASE_TAC >> rfs[])
     >- (EVERY_CASE_TAC >> fs[call_env_def, flush_state_def] >> rw[] >> fs[])
     >- (fs[jump_exc_def] >> EVERY_CASE_TAC >> rw[] >> fs[])
-    >- (fs[no_install_def2] >> EVERY_CASE_TAC >> rw[] >> fs[])
+    >- (fs[no_install_def] >> EVERY_CASE_TAC >> rw[] >> fs[])
     >- (EVERY_CASE_TAC >> fs[set_var_def] >> rw[] >> fs[])
-    >- (fs[no_install_def2])
+    >- (fs[no_install_def])
     >- (EVERY_CASE_TAC >> rw[] >> fs[])
     >- (EVERY_CASE_TAC >> rw[] >> fs[])
     >- (EVERY_CASE_TAC >> rw[] >> fs[] >> fs[ffiTheory.call_FFI_def] >>
@@ -4597,9 +4603,21 @@ Proof
       strip_tac >>
       drule share_inst_const >>
       simp[] )
-    >- (fs[no_install_def2, dec_clock_def, call_env_def, flush_state_def, push_env_def,
+    >- (fs[no_install_def, dec_clock_def, call_env_def, flush_state_def, push_env_def,
         cut_env_def, pop_env_def, set_var_def] >>
         EVERY_CASE_TAC >> rw[] >> fs[] >> metis_tac[no_install_find_code])
+QED
+
+Theorem get_code_labels_not_created:
+  !p x. (x IN get_code_labels p) <=>
+  (~ (not_created_subprogs (\sp. sp <> (wordLang$Call NONE (SOME x) [] NONE) /\
+    sp <> LocValue 0 x) p))
+Proof
+  ho_match_mp_tac get_code_labels_ind
+  \\ fs [not_created_subprogs_def]
+  \\ rw []
+  \\ every_case_tac \\ fs []
+  \\ EQ_TAC \\ rw [] \\ fs []
 QED
 
 (*** permute_swap for no_install & no_alloc ***)
@@ -4684,7 +4702,7 @@ Theorem permute_swap_lemma2:
 Proof
    ho_match_mp_tac (evaluate_ind |> Q.SPEC`UNCURRY P` |> SIMP_RULE (srw_ss())[] |> Q.GEN`P`) >>
    rw[] >> pairarg_tac >> rw[]
-   >~ [‘Alloc’] >- gvs[no_alloc_def2]
+   >~ [‘Alloc’] >- gvs[no_alloc_def]
    >~ [‘Move’]
    >- gvs[evaluate_def,set_vars_def,s_key_eq_refl,AllCaseEqs(),state_component_equality]
    >~ [‘Inst’]
@@ -4695,14 +4713,14 @@ Proof
    >~ [‘MustTerminate’]
    >- (gvs[evaluate_def, AllCaseEqs()] >>
        ntac 2 (pairarg_tac >> gvs[]) >>
-       gvs[AllCaseEqs(),no_alloc_def2,no_install_def2] >>
+       gvs[AllCaseEqs(),no_alloc_def,no_install_def] >>
        first_x_assum drule >>
        disch_then(qspec_then ‘perm’ mp_tac) >>
        rw[] >> simp[state_component_equality])
    >~ [‘Seq’]
    >- (gvs[evaluate_def, AllCaseEqs()] >>
        ntac 2 (pairarg_tac >> gvs[]) >>
-       gvs[AllCaseEqs(),no_alloc_def2,no_install_def2] >>
+       gvs[AllCaseEqs(),no_alloc_def,no_install_def] >>
        first_x_assum drule >>
        disch_then(qspec_then ‘perm’ mp_tac) >>
        rw[] >>
@@ -4731,12 +4749,12 @@ Proof
        metis_tac[PERM_fromAList])
    >~ [‘If’]
    >- (gvs[evaluate_def, AllCaseEqs(),get_var_imm_perm,get_var_imm_stack,
-           no_alloc_def2,no_install_def2] >>
+           no_alloc_def,no_install_def] >>
        first_x_assum drule >>
        disch_then(qspec_then ‘perm’ mp_tac) >>
        rw[] >> simp[state_component_equality])
    >~ [‘Install’]
-   >- gvs[no_install_def2]
+   >- gvs[no_install_def]
    >~ [‘Call’]
    >- (gvs[evaluate_def] >>
        PURE_TOP_CASE_TAC >> gvs[] >>
@@ -4873,14 +4891,14 @@ Proof
                    simp[] >>
                    disch_then $ ASSUME_TAC o GSYM >>
                    simp[] >>
-                   gvs[no_alloc_def2,no_install_def2])
+                   gvs[no_alloc_def,no_install_def])
                >- (first_x_assum match_mp_tac >>
                    simp[] >>
                    drule_then drule no_install_evaluate_const_code >>
                    simp[] >>
                    disch_then $ ASSUME_TAC o GSYM >>
                    simp[] >>
-                   gvs[no_alloc_def2,no_install_def2])) >>
+                   gvs[no_alloc_def,no_install_def])) >>
            PairCases_on ‘x'’ >>
            gvs[set_var_def,PULL_EXISTS,push_env_def,env_to_list_def] >>
            drule_all no_alloc_find_code >>
@@ -4910,14 +4928,14 @@ Proof
                simp[] >>
                disch_then $ ASSUME_TAC o GSYM >>
                simp[] >>
-               gvs[no_alloc_def2,no_install_def2])
+               gvs[no_alloc_def,no_install_def])
            >- (first_x_assum match_mp_tac >>
                simp[] >>
                drule_then drule no_install_evaluate_const_code >>
                simp[] >>
                disch_then $ ASSUME_TAC o GSYM >>
                simp[] >>
-               gvs[no_alloc_def2,no_install_def2]))
+               gvs[no_alloc_def,no_install_def]))
        >~ [‘evaluate _ = (SOME(Exception _ _),_)’]
        >- (gvs[call_env_def,dec_clock_def] >>
            ‘stack_size stack = stack_size st.stack’ by gvs[stack_size_perm] >>
@@ -4963,7 +4981,7 @@ Proof
            simp[] >>
            disch_then $ ASSUME_TAC o GSYM >>
            simp[] >>
-           gvs[no_alloc_def2,no_install_def2])
+           gvs[no_alloc_def,no_install_def])
       )
    >~ [`ShareInst`]
    >- (
@@ -5006,24 +5024,15 @@ QED
 
 (****** no_mt : no MustTerminate ******)
 
-val no_mt_def = Define `
-  (no_mt (MustTerminate p) = F) /\
-  (no_mt (Call ret _ _ handler) =
-     (case ret of
-      | NONE =>
-            (case handler of
-             | NONE => T
-             | SOME (_,ph,_,_) => no_mt ph)
-      | SOME (_,_,pr,_,_) =>
-            (case handler of
-             | NONE => no_mt pr
-             | SOME (_,ph,_,_) => no_mt ph /\ no_mt pr))) /\
-  (no_mt (Seq p1 p2) = (no_mt p1 /\ no_mt p2)) /\
-  (no_mt (If _ _ _ p1 p2) = (no_mt p1 /\ no_mt p2)) /\
-  (no_mt _ = T)
-`
+val no_mt_P = ``((<>) (MustTerminate Skip))``
 
-val no_mt_ind = theorem "no_mt_ind";
+Definition no_mt_subprogs_def:
+  no_mt p = not_created_subprogs ^no_mt_P p
+End
+
+Theorem no_mt_def = not_created_subprogs_P_def
+  |> ISPEC no_mt_P
+  |> REWRITE_RULE [GSYM no_mt_subprogs_def]
 
 val no_mt_code_def = Define `
   no_mt_code (code : (num # ('a wordLang$prog)) num_map) <=>
@@ -5042,22 +5051,15 @@ Proof
 QED
 
 (* no_share_inst: no ShareInst *)
-Definition no_share_inst_def:
-  (no_share_inst (ShareInst _ _ _) = F) /\
-  (no_share_inst (MustTerminate p) = no_share_inst p) ∧
-  (no_share_inst (Call ret _ _ handler) =
-     (case ret of
-      | NONE =>
-          (case handler of
-           | NONE => T
-           | SOME (_,ph,_,_) => no_share_inst ph)
-      | SOME (_,_,pr,_,_) =>
-          (case handler of
-           | NONE => no_share_inst pr
-           | SOME (_,ph,_,_) => no_share_inst ph /\ no_share_inst pr))) /\
-  (no_share_inst (Seq p1 p2) = (no_share_inst p1 /\ no_share_inst p2)) /\
-  (no_share_inst (If _ _ _ p1 p2) = (no_share_inst p1 /\ no_share_inst p2)) /\
-  (no_share_inst _ = T)
+
+val no_share_inst_P = ``((<>) (ShareInst ARB 0 (Var 0)))``
+
+Definition no_share_inst_subprogs_def:
+  no_share_inst p = not_created_subprogs ^no_share_inst_P p
 End
+
+Theorem no_share_inst_def = not_created_subprogs_P_def
+  |> ISPEC no_share_inst_P
+  |> REWRITE_RULE [GSYM no_share_inst_subprogs_def]
 
 val _ = export_theory();
